\documentclass{article}

\usepackage{amsmath}

\title{Homework}
\author{Farzad Sadeghi}
\date{1400/02/30}

\begin{document}
\maketitle
\section{Problem 1}

(a/b)-c+d*e-(a*e)\\
infix to postfix?\\
infix to prefix?\\
\begin{equation*}
  (a/b)-c+d*e-(a*e) = ((((a/b)-c)+(d*e))-(a*e))
\end{equation*}
infix to postfix:\\
\begin{equation*}
  ((((a/b)-c)+(d*e))-(a*e)) = ((((a/b)^/-c)^-+(d*e)^*)^+-(a*e)^*)^- = \underline{\bf a,b,/,c,-,d,e,*,+,a,e,*,-}
\end{equation*}
infix to prefix:\\
\begin{equation*}
  ((((a/b)-c)+(d*e))-(a*e)) = {}^-({}^+({}^-({}^/(a/b)-c)+{}^*(d*e))-{}^*(a*e)) = \underline{\bf -,+,-,/,a,b,c,*,d,e,*,a,e}
\end{equation*}

\end{document}
